SystemF2Effect: add store properties to kind judgement
Ignore-this: c5a153dbe60ce09e349c30f227a36dfe

darcs-hash:20130116040253-08f32-0c35e062c539f749abf323aa4e07483c85d56696

devel/Iron/Language/SystemF2Effect/Store/Prop.v
@@ -4,7 +4,8 @@
 Inductive stprop :=
  (* A region descriptor.
     One of these exists in the store for every live region in the store. *)
- | SRegion  : stprop.
+ | SRegion : nat -> stprop.
 
 
-Definition stprops := list stprop.
+Definition stprops 
+ := list stprop.
