devel/Iron/Language/SystemF2Effect/Type/KiJudge.v
@@ -2,6 +2,7 @@
 Require Export Iron.Language.SystemF2Effect.Type.Lift.
 Require Export Iron.Language.SystemF2Effect.Type.Wf.
 Require Export Iron.Language.SystemF2Effect.Type.Ty.
+Require Export Iron.Language.SystemF2Effect.Store.Prop.
 
 
 (* Only types of effect and closure kinds can be used in sums. *)
@@ -17,43 +18,43 @@ Hint Unfold appkind.
 
 
 (* Kinds judgement assigns a kind to a type *)
-Inductive KIND : kienv -> ty -> ki -> Prop :=
+Inductive KIND : kienv -> stprops -> ty -> ki -> Prop :=
   | KiCon
-    :  forall ke tc k
+    :  forall ke sp tc k
     ,  k = kindOfTyCon tc
-    -> KIND ke (TCon tc) k
+    -> KIND ke sp (TCon tc) k
 
   | KiCap
-    :  forall ke n
-    ,  KIND ke (TCap (TyCapRegion n)) KRegion
+    :  forall ke sp n
+    ,  KIND ke sp (TCap (TyCapRegion n)) KRegion
 
   | KiVar
-    :  forall ke i k
+    :  forall ke sp i k
     ,  get i ke = Some k
-    -> KIND ke (TVar i) k
+    -> KIND ke sp (TVar i) k
 
   | KiForall
-    :  forall ke k t
-    ,  KIND (ke :> k) t             KData
-    -> KIND ke        (TForall k t) KData
+    :  forall ke sp k t
+    ,  KIND (ke :> k) sp t KData
+    -> KIND ke        sp (TForall k t) KData
 
   | KiApp 
-    :  forall ke t1 t2 k11 k12
+    :  forall ke sp t1 t2 k11 k12
     ,  appkind k12
-    -> KIND ke t1 (KFun k11 k12)
-    -> KIND ke t2 k11
-    -> KIND ke (TApp t1 t2) k12
+    -> KIND ke sp t1 (KFun k11 k12)
+    -> KIND ke sp t2 k11
+    -> KIND ke sp (TApp t1 t2) k12
 
   | KiSum
-    :  forall ke k t1 t2
+    :  forall ke sp k t1 t2
     ,  sumkind k
-    -> KIND ke t1 k -> KIND ke t2 k
-    -> KIND ke (TSum t1 t2) k
+    -> KIND ke sp t1 k -> KIND ke sp t2 k
+    -> KIND ke sp (TSum t1 t2) k
 
   | KiBot
-    :  forall ke k
+    :  forall ke sp k
     ,  sumkind k
-    -> KIND ke (TBot k) k.
+    -> KIND ke sp (TBot k) k.
 
 Hint Constructors KIND.
 
@@ -62,33 +63,33 @@ Hint Constructors KIND.
 Ltac inverts_kind :=
  repeat 
   (match goal with 
-   | [ H: KIND _ (TCon _)    _   |- _ ] => inverts H
-   | [ H: KIND _ (TCap _)    _   |- _ ] => inverts H
-   | [ H: KIND _ (TVar _)    _   |- _ ] => inverts H
-   | [ H: KIND _ (TForall _ _) _ |- _ ] => inverts H
-   | [ H: KIND _ (TApp _ _) _    |- _ ] => inverts H
-   | [ H: KIND _ (TSum _ _) _    |- _ ] => inverts H
-   | [ H: KIND _ (TBot _ ) _     |- _ ] => inverts H
+   | [ H: KIND _ _ (TCon _)    _   |- _ ] => inverts H
+   | [ H: KIND _ _ (TCap _)    _   |- _ ] => inverts H
+   | [ H: KIND _ _ (TVar _)    _   |- _ ] => inverts H
+   | [ H: KIND _ _ (TForall _ _) _ |- _ ] => inverts H
+   | [ H: KIND _ _ (TApp _ _) _    |- _ ] => inverts H
+   | [ H: KIND _ _ (TSum _ _) _    |- _ ] => inverts H
+   | [ H: KIND _ _ (TBot _ ) _     |- _ ] => inverts H
    end).
 
 
 (********************************************************************)
 (* A well kinded type is well formed *)
 Lemma kind_wfT
- :  forall ke t k
- ,  KIND ke t k
- -> wfT  (length ke) t.
+ :  forall ke sp t k
+ ,  KIND   ke sp t k
+ -> wfT (length ke) t.
 Proof.
- intros ke t k HK. gen ke k.
+ intros ke sp t k HK. gen ke sp k.
  induction t; intros; inverts_kind; burn.
- lets D: IHt H3. burn.
+ lets D: IHt H4. burn.
 Qed.
 Hint Resolve kind_wfT.
 
 
 Lemma kind_wfT_Forall
- :  forall ks k ts
- ,  Forall (fun t => KIND ks t k) ts
+ :  forall ks sp k ts
+ ,  Forall (fun t => KIND ks sp t k) ts
  -> Forall (wfT (length ks)) ts.
 Proof.
  intros. nforall. eauto.
@@ -97,12 +98,12 @@ Hint Resolve kind_wfT_Forall.
 
 
 Lemma kind_wfT_Forall2
- :  forall (ke: kienv) ts ks
- ,  Forall2 (KIND ke) ts ks
- -> Forall (wfT (length ke)) ts.
+ :  forall  (ke: kienv) (sp: stprops) ts ks
+ ,  Forall2 (KIND ke sp) ts ks
+ -> Forall  (wfT (length ke)) ts.
 Proof.
  intros.
- eapply (Forall2_Forall_left (KIND ke)); burn.
+ eapply (Forall2_Forall_left (KIND ke sp)); burn.
 Qed.
 Hint Resolve kind_wfT_Forall2.
 
@@ -110,8 +111,8 @@ Hint Resolve kind_wfT_Forall2.
 (********************************************************************)
 (* Forms of types *)
 Lemma kind_region
- :  forall t
- ,  KIND nil t KRegion
+ :  forall t sp
+ ,  KIND nil sp t KRegion
  -> (exists n, t = TCap (TyCapRegion n)).
 Proof.
  intros.
@@ -132,8 +133,8 @@ Hint Resolve kind_region.
 (* If a type is well kinded in an empty environment,
    then that type is closed. *)
 Lemma kind_empty_is_closed
- :  forall t k
- ,  KIND nil t k 
+ :  forall sp t k
+ ,  KIND   nil sp t k 
  -> closedT t.
 Proof.
  intros. unfold closedT.
@@ -145,13 +146,13 @@ Hint Resolve kind_empty_is_closed.
 
 
 (********************************************************************)
-(* Weakening kind environments. *)
+(* Weaken kind environment in kind judgement. *)
 Lemma kind_kienv_insert
- :  forall ke ix t k1 k2
- ,  KIND ke t k1
- -> KIND (insert ix k2 ke) (liftTT 1 ix t) k1.
+ :  forall ke sp ix t k1 k2
+ ,  KIND   ke sp t k1
+ -> KIND   (insert ix k2 ke) sp (liftTT 1 ix t) k1.
 Proof.
- intros. gen ix ke k1.
+ intros. gen ix ke sp k1.
  induction t; intros; simpl; inverts_kind; eauto.
 
  Case "TVar".
@@ -164,12 +165,24 @@ Qed.
 
 
 Lemma kind_kienv_weaken
- :  forall ke t k1 k2
- ,  KIND  ke         t             k1
- -> KIND (ke :> k2) (liftTT 1 0 t) k1.
+ :  forall ke sp t k1 k2
+ ,  KIND   ke sp        t              k1
+ -> KIND  (ke :> k2) sp (liftTT 1 0 t) k1.
 Proof.
  intros.
  rrwrite (ke :> k2 = insert 0 k2 ke).
  apply kind_kienv_insert. auto.
 Qed.
 
+
+(********************************************************************)
+(* Weaken store properties in kind judgement. *)
+Lemma kind_stprops_snoc
+ : forall ke sp p t k
+ ,  KIND ke sp        t k
+ -> KIND ke (p <: sp) t k.
+Proof.
+ intros. gen ke k.
+ induction t; intros; inverts_kind; burn.
+Qed.  
+  
